%% dvips  -t landscape filename 
\documentclass[10pt]{article}  
\usepackage[a4paper,total={7.50in, 10.70in}]{geometry}
%%=================================================
\usepackage{amsmath,amsfonts,amsthm,xcolor}
%--------------
\usepackage{enumitem}
\setenumerate{label=\arabic*,leftmargin=*}
%%\usepackage{portland}   %% \landscape  \portrait ...
%%\usepackage{lscape}
\usepackage{multicol}
\setlength{\columnseprule}{0.5pt}
\setlength\columnsep{25pt}
\def\columnseprulecolor{\color{olive}}
%%------------------------------------------------------------------------
\usepackage{fancyhdr}
\pagestyle{fancy}
\fancyhf{}
%%\fancyheadoffset[RO,LE]{5pt}
\fancyheadoffset[RO,LE]{0pt}
\renewcommand{\headrulewidth}{0pt}
%%\fancyfoot[C]{\footnotesize\thepage}
\fancyfoot[L]{\scriptsize\sc Applied Statistics Lab, PNU}
\fancyfoot[R]{\scriptsize\sc \copyright\; Chanseok Park}
%%=================================================
\newenvironment{LIST}[1]{\begin{list}{}
                          { \settowidth{\labelwidth}{#1}
                            \setlength{\leftmargin}{\labelwidth}
                            \addtolength{\leftmargin}{\labelsep}
                            \setlength{\parsep}{0.5ex plus0.2ex minus0.2ex}
                            \setlength{\itemsep}{0ex plus0.2ex}
                            \renewcommand{\makelabel}[1]{##1\hfill}
                          }
                        }
                        {\end{list}}
\newenvironment{reflist}[1]{\begin{list}{}
    { \settowidth{\leftmargin}{#1} \setlength{\itemindent}{-\leftmargin}
      %%\addtolength{\leftmargin}{\labelsep}
      \setlength{\parsep}{0.5ex plus0.2ex minus0.2ex}
      \setlength{\itemsep}{0ex plus0.2ex}
    } } {\end{list}}
%%=================================================

%% \pagestyle{empty}
%===================================================================
\begin{document}       
%%==================================================================
%%\landscape
%%------------------------------------------------------------------
\setlength{\baselineskip}{15pt plus 0.3pt minus 0.2pt} %% not in preamble
%%------------------------------------------------------------------
\setcounter{section}{0}

%%\centerline{\shadowbox{\huge\sf Probability Distribution} }
\centerline{\textcolor{olive}{\fbox{\Huge\textsf{~Probability Distribution~} }} }

% MAIN PART
\smallskip
\begin{multicols}{2}
\begin{small}
\begin{enumerate}
\item \textcolor{red}{\bfseries\textsf{Binomial}}\,$(n,p)$, ~~ $(x=0,1,\ldots,n)$ \hfill 
      \textsf{R:}$x$\texttt{\color{red}binom}  \\
      $f(x) = \binom{n}{x}p^x (1-p)^{n-x}$\\
      $M(t)=(pe^t + 1-p)^n$\\
      $E(X)=np$, $\textrm{Var}(X) =np(1-p)$
      \begin{LIST}{\textsc{Note:}}
      \item[\textsc{Note:}] 
          $n\to\infty \text{~with~} \mu=np \Rightarrow \textrm{Poisson}(\mu)$ \\
          $F_{\textrm{Bin}(n,p)}(x) = F_{\textrm{Beta}(n-x,x+1)}(1-p)$ \\
          $F_{\text{Bin}(n,p)}(r-1)=1-F_{\text{NegBin}(r,p)}(n-r)$ \\
          $X_i\sim\mathrm{Bin}(n_i,p)$ $\Rightarrow$ 
                 $\sum X_i \sim \mathrm{Bin}\big(\sum n_i,p\big)$
      \end{LIST}
\item \textcolor{red}{\bfseries\textsf{Geometric}}\,$(p)$  \hfill \textsf{R:}$x$\texttt{\color{red}geom}  \\
      $f(x)=p(1-p)^x$, ~~ $(x=0,1,\ldots)$ \\
      $F(t)=1-(1-p)^{\lfloor t\rfloor+1}$, where 
              $\lfloor t\rfloor = \max\{m\in\mathbb{Z}: m \le t\}$ \\
      $S(t)=P[X\ge t] = (1-p)^{\lceil t\rceil}$ with 
              $\lceil t\rceil = \min\{m\in\mathbb{Z}: m \ge t\}$ \\
      $R(t)=P[X  > t] = (1-p)^{\lfloor t\rfloor+1}$ \\
      $M_X(t)=\displaystyle\frac{p}{1-(1-p)e^t}, \quad ( t<-\log (1-p) )$\\
      $E(X)=\displaystyle\frac{1-p}{p}$, $\textrm{Var}(X)=\displaystyle\frac{1-p}{p^2}$ 

      {\textcolor{red}{\rule{0.43\textwidth}{0.5pt}}}   %%--------

      $f(y)=p(1-p)^{y-1}$, ~~ $(y=1,2,\ldots)$  \\
      $F(t)=1-(1-p)^{\lfloor t\rfloor}$ \\
      $S(t)=P[Y\ge t] = (1-p)^{\lceil t\rceil - 1}$ \\  
      $R(t)=P[Y >  t] = (1-p)^{\lfloor t\rfloor}$ \\  
      $M_Y(t)=\displaystyle\frac{pe^t}{1-(1-p)e^t}, ~ ( t<-\log (1-p) )$\\
      $E(Y)= \displaystyle\frac{1}{p}$, $\textrm{Var}(Y)=\displaystyle\frac{1-p}{p^2}$ 

      {\textcolor{red}{\rule{0.43\textwidth}{0.5pt}}}   %%--------
      %% \centerline{\textcolor{red}{\rule{0.4\textwidth}{0.5pt}}}   %%--------

      \vspace{-2ex}
      \begin{LIST}{\textsc{Note:}}
      \item[\textsc{Note:}] 
  $\displaystyle\min_{1\le i\le n}(X_i) \sim \textrm{Geo}\left(1-(1-p)^n\right)$: 
                    self-reproducing
      \end{LIST}
\item \textcolor{red}{\bfseries\textsf{Hypergeometric}}\,$(N,M,n)$  \hfill \textsf{R:}$x$\texttt{\color{red}hyper} \\
      $f(x)=\displaystyle\frac{\binom{M}{x}\binom{N-M}{n-x}}{\binom{N}{n}}$,\\
              \hspace*{\fill}$(\max(0,M-(N-n)) \le x \le \min(n,M))$\\
      $E(X)=n \left(\displaystyle\frac{M}{N}\right)$,
                  $\textrm{Var}(X) = n\displaystyle\frac{M}{N}\frac{(N-M)(N-n)}{N (N-1)}$
\item \textcolor{red}{\bfseries\textsf{Negative Binomial}}\,$(r,p)$   \hfill \textsf{R:}$x$\texttt{\color{red}nbinom} \\
      $f(x)= \binom{r+x-1}{x} p^r (1-p)^x$, $(x=0,1,\ldots)$\\
      $M_X(t)=\left( \frac{\displaystyle p}{\displaystyle 1-(1-p)e^t} \right)^r$ \\
      $E(X) = r \frac{1-p}{p}, ~\textrm{Var}(X) = r \frac{1-p}{p^2} $ 

      %% \centerline{\textcolor{red}{\rule{0.4\textwidth}{0.5pt}}}   %%--------
      {\textcolor{red}{\rule{0.43\textwidth}{0.5pt}}}   %%--------

      $f(y)= \binom{y-1}{r-1} p^r (1-p)^{y-r}$, $(y=r,r+1,\ldots)$\\
      $M_Y(t)=\left( \frac{\displaystyle p e^t}{\displaystyle 1-(1-p)e^t} \right)^r$ \\
      $E(Y) = r \frac{1}{p}, ~\textrm{Var}(Y) = r\frac{1-p}{p^2} $ \\[-3ex]

      %% \centerline{\textcolor{red}{\rule{0.4\textwidth}{0.5pt}}}   %%--------
      {\textcolor{red}{\rule{0.43\textwidth}{0.5pt}}}   %%--------

      \vspace{-2ex}
      \begin{LIST}{\textsc{Note:}}
      \item[\textsc{Note:}] 
          $X = V_1+\cdots+V_r$, ($V_i\sim{\textrm{Geometric}}(p)$)\\
          $(1-x)^{-n}=\sum_{k=0}^{\infty} \binom{n+k-1}{k}x^k ~~ (|x|<1)$ \\
          $\mu=r(1-p), r\to\infty \Rightarrow \textrm{Poisson}(\mu)$ \\
          $X_i\sim\mathrm{NB}(r_i,p)$ $\Rightarrow$ $\sum X_i \sim \mathrm{NB}\big(\sum r_i,p\big)$ \\
          %% $F_{\text{Bin}(n,p)}(r-1)=1-F_{\text{NegBin}(r,p)}(n-r)$ \\
          $F_{\text{NB}(r,p)}(x) = F_{\text{Beta}(r, \lfloor x\rfloor+1)}(p)$ \\  %% See  \cite{Rider:1962}
          $F_{\text{NB}(r,p)}(n-r) = 1 - F_{\text{Bin}(n,p)}(r-1)$ 
      \end{LIST}

\item \textcolor{red}{\bfseries\textsf{Poisson}}\,$(\mu)$  \hfill \textsf{R:}$x$\texttt{\color{red}pois} \\
      $f(x)=\frac{\displaystyle e^{-\mu}\mu^x}{\displaystyle x!}$,~~ $(x=0,1,\ldots)$\\ 
      $M(t)=\exp\left( \mu(e^t -1) \right)$\\
      $E(X)=\mu$, $\textrm{Var}(X)=\mu$  
      \begin{LIST}{\textsc{Note:}}
      \item[\textsc{Note:}] 
      $X_i\sim\mathrm{Poi}(\mu_i)$ $\Rightarrow$ $\sum X_i \sim \mathrm{Poi}(\sum\mu_i)$  
          \begin{xxalignat}{2}
             P_{\textrm{Poi}(\mu)}[X\ge n]
               &= F_{\Gamma(n,1)}(\mu) = F_{\Gamma(n,\mu)}(1)  & \\
               &= F_{\chi^2_{2n}}(2\mu)  & 
          \end{xxalignat}
      \end{LIST}
      
\end{enumerate}
%%=============================================================

\vspace*{\fill}
%%==================================================================
%% \chapter{Continuous Distributions\label{SEC:continuousdistribution}}
%%=============================================================
\begin{enumerate}
\item \textcolor{red}{\bfseries\textsf{Beta}}\,$(\alpha,\beta)$,~~  
       $(\alpha>0,\beta>0)$ \hfill \textsf{R:}$x$\texttt{\color{red}beta} \\
      $f(x)=\frac{\displaystyle \Gamma(\alpha+\beta)}{\displaystyle\Gamma(\alpha)\Gamma(\beta)}
            x^{\alpha-1}(1-x)^{\beta-1},~(0<x<1)$ \\
      $M(t) = 1 + \sum_{k=1}^{\infty}\left(\prod_{r=1}^{k-1}\frac{\alpha+r}{\alpha+\beta+r}\right)
              \frac{t^k}{k!}$\\
      $E(X)=\frac{\displaystyle \alpha}{\displaystyle \alpha+\beta}$,~
            $\textrm{Var}(X) =\frac{\displaystyle\alpha\beta}{\displaystyle(\alpha+\beta+1)(\alpha+\beta)^2}$
      \begin{LIST}{\textsc{Note:}}
      \item[\textsc{Note:}] $F_{\textrm{Beta}(n-x,x+1)}(1-p)=F_{\textrm{Bin}(n,p)}(x)$
      \end{LIST}

\item \textcolor{red}{\bfseries\textsf{BS}}\,$(\alpha,\beta)$,~~$(\alpha>0,\beta>0)$: 
   Birnbaum-Saunders \hfill \\
      $f(t)= {\frac{1}{2{\alpha}{\beta}}} \sqrt{\frac{\beta}{t}} \Big( 1 + {\frac{\beta}{t}} \Big)
         \phi\Big[\frac{1}{\alpha}\Big(\sqrt{\frac{t}{\beta}}-\sqrt{\frac{\beta}{t}} \Big)\Big],~(t>0)$\\
      $F(t) = \Phi \Big[ \frac{1}{\alpha}
            \Big( \sqrt{\frac{t}{\beta}}-\sqrt{\frac{\beta}{t}} \Big) \Big]$
% \\     $F^{-1}(p) = \frac{1}{4} 
%           \Big[ 
%   \alpha\sqrt{\beta}\Phi^{-1}(p)+\sqrt{\alpha^2\beta\{\Phi^{-1}(p)\}^2+4\beta}
%            \Big]^2$ \\
\begin{xxalignat}{2}
     F^{-1}(p) &= \frac{1}{4}  %hhhhhhhhhh
     \Big[ 
     \alpha\sqrt{\beta}\Phi^{-1}(p)+\sqrt{\alpha^2\beta\{\Phi^{-1}(p)\}^2+4\beta}
     \Big]^2 \\
      &= \beta\Big\{ 1+\gamma(p)^2 +\gamma(p)\sqrt{\gamma(p)^2+2} \Big\}, \\
      &\quad ~\text{where}~ \gamma(p)=\alpha\Phi^{-1}(p)/\sqrt{2}
\end{xxalignat}
      $E(T)= \beta(1+\frac{1}{2}\alpha^2)$, ~   
      $\textrm{Var}(T) = (\alpha\beta)^2(1+\frac{5}{4}\alpha^2)$
      \begin{LIST}{\textsc{Note:}}
      \item[\textsc{Note:}] 
     $\mathrm{median}(T)=\beta$, $cT \sim \textrm{BS}(\alpha,c\beta)$, 
     $T^{-1} \sim \textrm{BS}(\alpha,\beta^{-1})$ \\
     $X=\Big( \sqrt{\frac{T}{\beta}}-\sqrt{\frac{\beta}{T}} \, \Big) 
             \sim N(0,\alpha^2)$ \\
     $\log T \sim \textrm{sinh-Normal}(\log\beta,\alpha)$
      \end{LIST}

\item \textcolor{red}{\bfseries\textsf{Cauchy}}\,$(\alpha,\beta)$ \hfill \textsf{R:}$x$\texttt{\color{red}cauchy} \\
      $f(x) = \displaystyle\frac{\beta}{\pi} \frac{1}{\beta^2+(x-\alpha)^2}$\\
      $F(x) = \displaystyle\frac{1}{\pi}\left[\arctan\left(\frac{x-\alpha}{\beta}\right)
              + \frac{\pi}{2} \right]$ \\
      $\phi(t) = \exp(it\alpha-\beta|t|)$
      \begin{LIST}{\textsc{Note:}}
      \item[\textsc{Note:}] Cauchy$(0,1) = t(1)$\\
              $X,Y \sim N(0,1) \Rightarrow X/Y \sim \textrm{Cauchy}(0,1)$\\
              $cX \sim  \textrm{Cauchy}(c\alpha,c\beta)$\\
              $X_i \sim \textrm{Cauchy}(\alpha,\beta) \Rightarrow 
                \frac{1}{n}\sum X_i \sim \textrm{Cauchy}(\alpha,\beta)$ 
      \end{LIST}
\item \textcolor{red}{\bfseries\textsf{Chi Squared}}\,$(n)$ \hfill \textsf{R:}$x$\texttt{\color{red}chisq}  \\
      $f(x) = \displaystyle\frac{1}{\Gamma(n/2) 2^{n/2}} x^{n/2-1} e^{-x/2}$, $(x \ge 0)$\\
      $E(X)=n$, $\textrm{Var}(X)=2n$\\
      $M(t) = \left(\frac{1}{1-2t}\right)^{n/2},\quad (t < \frac{1}{2})$\\
      $E(X^m)=2^n \Gamma(m+n/2)/\Gamma(n/2)$ 
      \begin{LIST}{\textsc{Note:}}
      \item[\textsc{Note:}] 
           $\chi^2(n)=\textrm{Gamma}(n/2,2)$ \\
           $\chi^2(2)=\textrm{Exponential}(\beta=2)$ \\
           $X_i \sim \chi^2(n_i) \Rightarrow \sum X_i \sim \chi^2(\sum n_i)$ \\
           $X_i \sim N(0,1) \Rightarrow \sum_{i=1}^{n}X_i^2 \sim \chi^2(n)$\\
           $F_{\chi^2(p+2)}(x)=F_{\chi^2(p)}(x)-2xf_{\chi^2(p)}(x)/p$\\
           $F_{\chi^2(1)}(x)=2\Phi(\sqrt{x})-1$\\
           $F_{\chi^2(2)}(x)=1-\sqrt{2\pi}\phi(\sqrt{x})$\\
           $F_{\chi^2(3)}(x)=2\Phi(\sqrt{x})-1-2\sqrt{x}\phi(\sqrt{x})$
      \end{LIST}

\item \textcolor{red}{\bfseries\textsf{Exponential}}\,$(\theta)$ \hfill\textsf{R:}$x$\texttt{\color{red}exp}\\
      $f(x) = \displaystyle\frac{1}{\theta} e^{-x/\theta}$ $(x\ge0,~ \theta>0)$\\
      $F(x) = 1 - e^{-x/\theta}$ \\
      $M(t) = \displaystyle\frac{1}{1-\theta t}$, $(t < \frac{1}{\theta})$ \\
      $E(X)=\theta, \textrm{Var}(X)=\theta^2$
      \begin{LIST}{\textsc{Note:}}
      \item[\textsc{Note:}] Memoryless property\\
            $cX \sim \textrm{Exponential}(c\theta)$\\
            $\sum X_i \sim\mathrm{Gamma}(n,\theta)$\\
            $\displaystyle\min_{1\le i\le n}(X_i) \sim \textrm{Exponential}(\theta/n)$: self-reproducing\\
            $Y = X^{1/\alpha} \sim \textrm{Weibull}(\alpha,\theta)$\\
            $Y = \sqrt{2X/\theta} \sim \textrm{Rayleigh}(1)$\\
            $Y = \alpha-\gamma\log(X/\theta) \sim \textrm{Gumbel}(\alpha,\gamma)$
      \end{LIST}

\item $\textcolor{red}{\textbf{\textsl{F}}}\,(m,n)$ \hfill \textsf{R:}$x$\texttt{\color{red}f}  \\
      $F(m,n)=\displaystyle\frac{\chi^2_m/m}{\chi^2_n/n}$\\ 
      $E(X) = \displaystyle\frac{n}{n-2}~~(n>2)$,\\  
      $\textrm{Var}(X)=2\left(\displaystyle\frac{n}{n-2}\right)^2\displaystyle\frac{m+n-2}{m(n-4)}~(n>4)$
      \begin{LIST}{\textsc{Note:}}
      \item[\textsc{Note:}] $\left[F(m,n)\right]^{-1} = F(n,m)$\\
           $F_{1-\alpha}(m,n)=\left[F_{\alpha}(n,m)\right]^{-1}$ \\
           $F(1,k) = t^2(k)$   \\
           %% The following is from Theorem 5.3.8 on page 225 of Casella & Berger (2001)
           If $X \sim F(m,n)$, $mX/(mX+n) \sim \mathrm{Beta}(\frac{m}{2},\frac{n}{2})$. 
      \end{LIST}
\item \textcolor{red}{\bfseries\textsf{Gamma}}\,$(\alpha,\theta)$ \hfill \textsf{R:}$x$\texttt{\color{red}gamma} \\
      $f(x)=\frac{\displaystyle 1}{\displaystyle \Gamma(\alpha)\theta^\alpha}
                                 x^{\alpha-1} \exp(-x/\theta),~(0 < x<\infty)$\\
      $M(t)=(1-\theta t)^{-\alpha}$ $(t<1/\theta)$ \\
      $E(X)=\alpha\theta$, $\textrm{Var}(X)=\alpha\theta^2$ 
      \begin{LIST}{\textsc{Note:}}
      \item[\textsc{Note:}] $X\sim\textrm{Gamma}(n,\theta)=\textrm{Erlang}(n,\theta)$\\
             $X = V_1+\cdots+V_{n}$, ($V_i\sim{\textrm{Exponential}}(\theta)$)\\
             $2X/\theta \sim \chi^2(2n)$ 

            \vspace{-3ex}
            \begin{xxalignat}{2}
                F_X(x)&=1-\displaystyle\sum_{k=0}^{n-1}(\displaystyle\frac{x}{\theta})^k\frac{e^{-x/\theta}}{k!}& \\
                      &=\displaystyle\sum_{k=n}^{\infty}(\displaystyle\frac{x}{\theta})^k\frac{e^{-x/\theta}}{k!}& 
            \end{xxalignat}
             $\mathrm{Gamma}(n/2,2)=\chi^2(n)$,~  ${\Gamma}(1/2)=\sqrt{\pi}$\\
             $X_i \!\sim\! \mathrm{Gamma}(\alpha_i,\theta) \!\Rightarrow\! 
              \sum_{i=1}^{r} \!\!X_i \!\sim\! 
                      \mathrm{Gamma}(\sum_{i=1}^{r}\! \alpha_i,\theta)$\\
             $X/d \sim \mathrm{Gamma}(\alpha,\theta/d)$\\
             $E[X^c]=\Gamma(\alpha+c)\theta^c/\Gamma(\alpha)~(c>-\alpha)$
      \end{LIST}

\item \textcolor{red}{\bfseries\textsf{Laplace}}\,$(\mu,\sigma)$: Double Exponential \\
      $f(x) = \frac{1}{2\sigma} e^{-|x-\mu|/\sigma}$ \\
      $F(x) = \left\{ \begin{array}{l@{\qquad}l}
              \frac{1}{2} e^{-|x-\mu|/\sigma} & (x<\mu) \\
            1-\frac{1}{2} e^{-|x-\mu|/\sigma} & (x \ge \mu) \\
                      \end{array} \right.$ \\
      $M(t)=\displaystyle\frac{e^{\mu t}}{1-(\sigma t)^2}$, $(|t|<\frac{1}{\sigma})$ \\
      $E(X) = \mathrm{median}(X) = \mu$, $\textrm{Var}(X)=2\sigma^2$ 

\item \textcolor{red}{\bfseries\textsf{Logistic}},$(\mu,\beta)$ \hfill \textsf{R:}$x$\texttt{\color{red}logis} \\
      $f(x) = \displaystyle\frac{e^{-(x-\mu)/\beta}}{\beta[1+e^{-(x-\mu)/\beta}]^2}
            = \displaystyle\frac{1}{2\beta\left[1+\cosh\left(\frac{x-\alpha}{\beta}\right)\right]}$\\
      $F(x) = \displaystyle\frac{1}{1+e^{-(x-\mu)/\beta}}$\\
      $M(t) = e^{\mu t}\Gamma(1-\beta t) \Gamma(1+\beta t)$, $|t| < \frac{1}{\beta}$\\
      $E(X)=\mathrm{median}(X)=\mu, \textrm{Var}(X)=\frac{\pi^2\beta^2}{3}$

\item \textcolor{red}{\bfseries\textsf{Lognormal}}\,$(\mu,\sigma^2)$ \hfill \textsf{R:}$x$\texttt{\color{red}lnorm} \\
      $f(x)=\frac{\displaystyle 1}{\displaystyle \sigma\sqrt{2\pi}x}
            \exp(-\frac{1}{2}(\frac{\log(x)-\mu}{\sigma})^2)$\\
      $E(X^k)=e^{k\mu+k^2 \sigma^2/2}, \textrm{Var}(X)=e^{2(\mu+\sigma^2)}-e^{2\mu+\sigma^2}$
      \begin{LIST}{\textsc{Note:}}
      \item[\textsc{Note:}]
      $F_{logN(\mu,\sigma^2)}(x)=F_{N(\mu,\sigma^2)}(\log x)
         =\Phi\big( \frac{\log x-\mu}{\sigma} \big)$ \\
      Self-reproducing under multiplication and division
      \end{LIST}

\item \textcolor{red}{\bfseries\textsf{Normal}}\,$(\mu,\sigma^2)$\hfill\textsf{R:}$x$\texttt{\color{red}norm}\\
      $f(x)=\frac{\displaystyle 1}{\displaystyle \sigma\sqrt{2\pi}}
                              \exp(-\frac{1}{2}(\frac{x-\mu}{\sigma})^2)$\\
      $ M(t) = \exp(\mu t+\frac{1}{2}\sigma^2 t^2)$
      \begin{LIST}{\textsc{Note:}}
      \item[\textsc{Note:}]
           If $X \sim N(\mu,\sigma^2)$,  $Y=e^{X} \sim logN(\mu,\sigma^2)$
           \begin{xxalignat}{2}
   F_{N(0,1)}(x)&=\frac{1}{2}+\frac{1}{2}\textrm{sign}(x)F_{\Gamma(1/2,1)}(\frac{1}{2}x^2)&\\
                &=\frac{1}{2}+\frac{1}{2}\textrm{sign}(x)F_{\chi^2(1)}(x)&
           \end{xxalignat}
      \item $\phi'(z)=-z\phi(z)$, $\phi''(z)=(z^2-1)\phi(z)$
      \item $E(X^3)=\mu^3+3\mu\sigma^2$, $E(X^4)=\mu^4+6\mu^2\sigma^2+3\sigma^4$
      \end{LIST}

\item \textcolor{red}{\bfseries\textsf{Rayleigh}}\,$(\beta)$ \\
      $f(x) = \displaystyle\frac{x}{\beta^2} \exp\Big(-\frac{x^2}{2\beta^2} \Big)$ \\
      $F(x) = 1 - \displaystyle\exp\Big(-\frac{x^2}{2\beta^2} \Big)$ \\
      $E(X)   = \beta \sqrt{\pi/2}$,
      $E(X^k) = (\sqrt{2}\beta)^k \frac{k}{2} \Gamma(\frac{k}{2})$ \\
      $\mathrm{median}(X)=\beta\sqrt{2\ln2}$ \\
      $\textrm{Var}(X)= (2-\pi/2) \beta^2$ 
      \begin{LIST}{\textsc{Note:}}
      \item[\textsc{Note:}]
           $\textrm{Rayleigh}(\beta) = \textrm{Weibull}(2,2\beta^2)$ \\
           $cX \sim  \textrm{Rayleigh}(c\beta)$ \\
           $(X/\beta)^2 \sim  \chi^2(2)$  \\
        $X^2 \sim\textrm{Exponential}({2\beta^2}) = \mathrm{Gamma}(1,2\beta^2)$\\
           $\displaystyle\min_{1\le i\le n}(X_i) \sim \textrm{Rayleigh}(\beta/\sqrt{n})$: self-reproducing 
      \end{LIST}

\item \textcolor{red}{\bfseries\textsf{Slash}}\,$(\alpha,\beta)$ \\
      $f(x)=\frac{1}{\sqrt{2\pi}(x-\alpha)^2/\beta^2}
            \big(1-\exp(-\frac{1}{2}(\frac{x-\alpha}{\beta})^2)\big)$\\
      $F(x)=\Phi\big(\frac{x-\alpha}{\beta}\big)-
            (\frac{x-\alpha}{\beta}\big)f_{\mathrm{Slash}(0,1)}(\frac{x-\alpha}{\beta}\big)$
      \begin{LIST}{\textsc{Note:}}
      \item[\textsc{Note:}]
           $X=\alpha+\beta\displaystyle\frac{Z}{U}$, \\
            where $Z\sim N(0,1)$ and $U\sim \textrm{Uniform}(0,1)$.
      \end{LIST}
\item \textcolor{red}{\bfseries\textsf{Student}}\,$t(k)$ \hfill \textsf{R:}$x$\texttt{\color{red}t} \\
      $f(x)=\displaystyle\frac{\Gamma((k+1)/2)}{\Gamma(k/2)}
         \frac{1}{\sqrt{k\pi}}\Big(1+\frac{x^2}{k}\Big)^{-(k+1)/2}$, $(k \ge 1)$\\
      $E(X)=0~(k>1)$, $\textrm{Var}(X) = k/(k-2)~(k>2)$ \\[-3ex]
      \begin{LIST}{\textsc{Note:}}
      \item[\textsc{Note:}]
           $X\sim\displaystyle\frac{N(0,1)}{\sqrt{\chi^2_k/k}}$, ~~~ 
           $F_{\alpha}(1,k)=t_{\alpha/2}(k)^2$
           \begin{xxalignat}{3}
           F_{t(k)}(x)&=1-\frac{1}{2}F_{\textrm{Beta}(k/2,1/2)}(\textstyle\frac{k}{k+x^2})&(x\ge 0)& \\
                        &=\frac{1}{2}F_{\textrm{Beta}(k/2,1/2)}(\textstyle\frac{k}{k+x^2})&(x < 0)& 
           \end{xxalignat}
      \end{LIST}

\item \textcolor{red}{\bfseries\textsf{Uniform}}\,$(a,b)$ \hfill \textsf{R:}$x$\texttt{\color{red}unif} \\
      $f(x)=\displaystyle\frac{1}{b-a}$\\
      $M(t)=\displaystyle\frac{e^{tb}-e^{ta}}{t(b-a)}$, $(t\neq0)$\\
      $E(X)=\mathrm{median}(X)=\displaystyle\frac{a+b}{2}$, $\textrm{Var}(X) = \displaystyle\frac{(b-a)^2}{12}$
      \begin{LIST}{\textsc{Note:}}
      \item[\textsc{Note:}] 
           $X\sim \textrm{Uniform}(0,1)$, $-\log X \sim \textrm{Exponential}(1)$
      \end{LIST}

\item \textcolor{red}{\bfseries\textsf{Wald}}\,$(\mu,\lambda)$: Inverse Gaussian\,(IG)  \hfill 
      \textsf{R:}$x$\texttt{\textcolor{red}{invgauss}\{statmod\}} \\
      $f(x;\mu,\lambda) = \sqrt{\frac{\lambda}{2\pi x^3}}
             \exp\left[-\lambda\frac{(x-\mu)^2}{2\mu^2 x}\right]
  =\sqrt{\frac{\lambda}{x^3}} \phi\Big(\sqrt{\frac{\lambda}{x}}\frac{x-\mu}{\mu}\Big)$\\
      $E(X)=\mu$, $\textrm{Var}(X)=\mu^3/\lambda$\\
      $F(x) = \Phi\Big( \sqrt{\frac{\lambda}{x}} \frac{x-\mu}{\mu}\Big)
            +\exp\Big(\frac{2\lambda}{\mu}\Big) 
              \Phi\Big(-\sqrt{\frac{\lambda}{x}} \frac{x+\mu}{\mu} \Big) $ \\
    $M(t)=\exp\Big[  \frac{\lambda}{\mu}
     \big( 1-\sqrt{1-{2\mu^2 t}/{\lambda}}\,\big)  \Big]$  \\
   $\hat{\mu}_{\textrm{mle}}=\bar{X}$, 
   $\hat{\lambda}_{\textrm{mle}}=
      \Big[ \frac{1}{n}\sum\big\{ X_i^{-1}-\bar{X}^{-1}\big\}\Big]^{-1}$.
  %%$\hat{\lambda}=\Big[ \sum X_i^{-1}/n-\bar{X}^{-1}\Big]^{-1}$.
      \begin{LIST}{\textsc{Note:}}
      \item[\textsc{Note:}] 
       $\lambda(X-\mu)^2/(\mu^2 X) \sim \chi^2(1)$ \\
       $X_i\sim\textrm{IG}(\mu,\lambda)$ $\!\Rightarrow\!$
       $k X_i \sim\textrm{IG}(k\mu,k\lambda)$,    \\
       ${\qquad\qquad}$ $\sum X_i \sim\textrm{IG}(n\mu, n^2\lambda)$,  
       $n\lambda/\hat{\lambda}_{\textrm{mle}} \sim \chi^2(n-1)$
      \end{LIST}

\item \textcolor{red}{\bfseries\textsf{Weibull}}\,$(\alpha,\theta)$ \hfill \textsf{R:}$x$\texttt{\color{red}weibull}  \\
      $f(x)=\displaystyle\frac{\alpha}{\theta} \Big(\frac{x}{\theta}\Big)^{\alpha-1} 
                \exp\big(-({x}/{\theta})^{\alpha} \big)$,
            $(x\ge0, \alpha>0, \theta>0)$  \\
      $F(x)=1-\exp\big( -({x}/{\theta})^{\alpha} \big)$\\
      $E(X^k) = \theta^k \Gamma(1+\frac{k}{\alpha})$,  ~
         $\mathrm{median}(X) =  \theta\,(\ln2)^{1/\alpha}$ \\
      $\textrm{Var}(X)= \theta^2
            \Big[\Gamma(1+\frac{2}{\alpha})-\Gamma^2(1+\frac{1}{\alpha})\Big]$
      \begin{LIST}{\textsc{Note:}}
      \item[\textsc{Note:}] 
           $\theta = 1-e^{-1} \approx$  63.2\% percentile \\
           $Y = X^{\alpha} \sim \textrm{Exponential}(\theta^{\alpha})$\\
           $\textrm{Weibull}(1,\theta)=\textrm{Exponential}(\theta)$  \\
           $\textrm{Weibull}(2, \sqrt{2}\theta)=\textrm{Rayleigh}(\theta)$  \\
           $\displaystyle\min_{1\le i\le n}(X_i)$ $\sim$
                   $\textrm{Weibull}(\alpha,\theta/{n}^{1/\alpha})$: self-reproducing 
      \end{LIST}

%=======================================================================
\end{enumerate} 
\end{small}
\end{multicols}
% END of MAIN PART




%%==================================================================
\end{document}             % End of document.
%%==================================================================
